Reap/Tactic/Syntax.lean
@@ -215,4 +215,4 @@ elab "reapMCTS" : tactic => do
   let opts ← Lean.getOptions
   let maxGoals := reap.max_goals.get opts
   let maxSteps := reap.max_steps.get opts
-  Reap.TreeSearch.reapMCTS TacticGenerator.generateTacticsWithPremises TacticGenerator.generateValue maxGoals maxSteps
+  Reap.TreeSearch.reapMCTS TacticGenerator.generatePolicyValue maxGoals maxSteps
